MRiscX/Hoare/EvalLabelInHoare.lean
@@ -1,4 +1,3 @@
-import MRiscX.AbstractSyntax.AbstractSyntax
 import MRiscX.Elab.HandleExpr
 open Lean Elab
 
